Added insertion to BST.

Bitree.v
@@ -12,17 +12,18 @@ Inductive tree : Set :=
 Inductive lt_tree : nat -> tree -> Prop :=
   lt_leaf : forall (n   : nat), lt_tree n leaf
 | lt_node : forall (n m : nat) (l r : tree), 
-   m < n -> lt_tree n l -> lt_tree n r -> lt_tree n (node n l r).
+   m < n -> lt_tree n l -> lt_tree n r -> lt_tree n (node m l r).
 
 Inductive gt_tree : nat -> tree -> Prop :=
   gt_leaf : forall (n   : nat), gt_tree n leaf
 | gt_node : forall (n m : nat) (l r : tree), 
-   m > n -> gt_tree n l -> gt_tree n r -> gt_tree n (node n l r).
+   m > n -> gt_tree n l -> gt_tree n r -> gt_tree n (node m l r).
 
 Inductive is_search_tree : tree -> Prop :=
   st_leaf : is_search_tree leaf
 | st_node : forall (n : nat) (l r : tree), 
-   lt_tree n l -> gt_tree n r -> is_search_tree (node n l r).
+   lt_tree n l -> is_search_tree l -> gt_tree n r -> is_search_tree r ->
+   is_search_tree (node n l r).
 
 Inductive contains : nat -> tree -> Prop :=
   root_contains : forall (n : nat) (l r : tree), contains n (node n l r)
@@ -33,19 +34,99 @@ Inductive contains : nat -> tree -> Prop :=
 
 Hint Constructors lt_tree gt_tree is_search_tree contains.
 
+Lemma subtree_is_search_tree n l r : is_search_tree (node n l r) ->
+                                     is_search_tree l /\ lt_tree n l /\
+                                     is_search_tree r /\ gt_tree n r.
+Proof. admit. Qed.
+
+Lemma containsSmall n t : (forall x, contains x t -> n < x) -> gt_tree n t.
+Proof. admit. Qed.
+
+Lemma containsBig n t : (forall x, contains x t -> n > x) -> lt_tree n t.
+Proof. admit. Qed.
+
+Lemma containsInLT n t : lt_tree n t -> forall x, contains x t -> n > x.
+Proof. admit. Qed.
+
+Lemma containsInGT n t : gt_tree n t -> forall x, contains x t -> n < x.
+Proof. admit. Qed.
+
+Lemma lt_tree_trans n m t : lt_tree n t -> n < m -> lt_tree m t.
+Proof. admit. Qed.
+
+Lemma gt_tree_trans n m t : gt_tree n t -> n > m -> gt_tree m t.
+Proof. admit. Qed.
+
 Definition add_in_search_tree : forall (t : tree) (n : nat),
   is_search_tree t -> 
   {t' | is_search_tree t' & 
-        contains n t' /\ forall (m : nat),
-        contains m t -> contains m t'
+        contains n t' /\ (forall (m : nat), contains m t -> contains m t')
+                      /\ (forall (m : nat), contains m t' -> m = n \/ contains m t)
   }.
 Proof.
-  intros. induction t. exists (node n leaf leaf); auto. 
-    assert (L: is_search_tree t1). 
-      
-    remember (lt_eq_lt_dec n n0) as B. inversion B. inversion H0.
-      
-
+  intro t. induction t.
+    intros m H1. exists (node m leaf leaf); auto.
+      split; auto. split; auto.
+        intros n H2. inversion H2; auto. 
+    intros m H1.
+      remember (subtree_is_search_tree _ _ _ H1) as H2.
+        inversion H2. inversion H0. inversion H4.
+          remember (lt_eq_lt_dec n m) as B1.
+            inversion B1.
+              inversion H7.
+                remember (IHt2 m H5) as B2.
+                  inversion B2.
+                    exists (node n t1 x).
+                      apply (st_node n t1 x); try assumption.
+                        apply (containsSmall n x).
+                          intros p C1. inversion H10. inversion H12.
+                            remember (H14 p C1) as C2.
+                              inversion C2. rewrite H15. assumption.
+                                apply (containsInGT n t2 H6). assumption.
+                      split.
+                        apply right_contains.
+                          inversion H10. assumption.
+                        split.
+                          intros p C1. inversion C1. constructor.
+                            apply left_contains. assumption.
+                            apply right_contains.
+                              inversion H10. inversion H17.
+                                apply H18. assumption.
+                          intros p C1. inversion C1. right. constructor. 
+                            right. apply left_contains. assumption.
+                              inversion H10. inversion H17.
+                                remember (H19 p H13) as C2.
+                                  inversion C2.
+                                    left. assumption.
+                                    right. apply right_contains. assumption.
+                exists (node n t1 t2). assumption.
+                  rewrite<-H8. auto.
+                remember (IHt1 m H) as B2.
+                  inversion B2.
+                    exists (node n x t2).
+                      apply (st_node n x t2); try assumption.
+                        apply (containsBig n x).
+                          intros p C1. inversion H9. inversion H11.
+                            remember (H13 p C1) as C2.
+                              inversion C2. rewrite H14. assumption.
+                                apply (containsInLT n t1 H3). assumption.
+                      split.
+                        apply left_contains.
+                          inversion H9. assumption.
+                        split.
+                          intros p C1. inversion C1. constructor.
+                            apply left_contains.
+                              inversion H9. inversion H16.
+                                apply H17. assumption.
+                            apply right_contains. assumption.
+                          intros p C1. inversion C1. right. constructor. 
+                            inversion H9. inversion H16.
+                              remember (H18 p H12) as C2.
+                                inversion C2. left. assumption.
+                                  right. apply left_contains. assumption.
+                            right. apply right_contains. assumption.
+Defined. 
+            
 Fixpoint height (t: tree) : nat := 
   match t with
   | leaf => 0
